---
layout: single
title: "Longest Common Subsequence"
date: 2024-03-13 20:48:54 +0800
categories: algo
tags: dp leetcode 
collection: 2024
classes: wide

toc: true
toc_label: "Content Outline"
toc_icon: "cog"
toc_sticky: true

---


## [1143. Longest Common Subsequence](https://leetcode.com/problems/longest-common-subsequence/)

Given two strings `text1` and `text2`, return *the length of their longest **common subsequence**.* If there is no **common subsequence**, return `0`.

A **subsequence** of a string is a new string generated from the original string with some characters (can be none) deleted without changing the relative order of the remaining characters.

- For example, `"ace"` is a subsequence of `"abcde"`.

A **common subsequence** of two strings is a subsequence that is common to both strings.

 

**Example 1:**

```
Input: text1 = "abcde", text2 = "ace" 
Output: 3  
Explanation: The longest common subsequence is "ace" and its length is 3.
```

**Example 2:**

```
Input: text1 = "abc", text2 = "abc"
Output: 3
Explanation: The longest common subsequence is "abc" and its length is 3.
```

**Example 3:**

```
Input: text1 = "abc", text2 = "def"
Output: 0
Explanation: There is no such common subsequence, so the result is 0.
```

 

**Constraints:**

- `1 <= text1.length, text2.length <= 1000`
- `text1` and `text2` consist of only lowercase English characters.



## Analysis

​	It's all about **Selection** or **Ignore** certain index of the sequence. Suppose we get the last letter in the sequence **s** and **t**,  the letter are **x** and **y**. There are four cases

1. [] 

2. [x] 

3. [y]

4. [x, y]

   So we can deduce the following function




### 1. dfs function


$$
dfs(i,j) =  \begin{cases}      
    	max(df(i-1, j), dfs(i, j-1), dfs(i-1, j-1)+1) & \text{s[i] = t[j]}\\      
    	max(dfs(i-1, j), dfs(i, j-1), dfs(i-1, j-1))  & \text{s[i] != t[j]}\\    
     \end{cases}
$$

$$
   dfs(i,j) = max(dfs(i-1, j), dfs(i, j-1), dfs(i-1, j-1) + (s[i]=t[j]))
$$

$$
dfs(i,j) =  \begin{cases}
      dfs(i-1, j-1)+1 & \text{s[i] = t[j]}\\
      max(dfs(i-1, j), dfs(i, j-1)) & \text{s[i] != t[j]}\\

    \end{cases}
$$

### 2. dp function

$$
f(i,j) =  \begin{cases}      
	f[i-1][j-1]+1 & \text{s[i] = t[j]}\\      
	max(f[i-1][j], f[i][j-1) & \text{s[i] != t[j]}\\   
	\end{cases}
$$

$$
f(i+1,j+1) =  \begin{cases}      
	f[i][j]+1 & \text{s[i+1] = t[j+1]}\\      
	max(f[i][j+1], f[i+1][j) & \text{s[i+1] != t[j+1]}\\   
	\end{cases}
$$


## Solutions 



### 1. DFS way

```py
class Solution:
    def longestCommonSubsequence(self, s: str, t: str) -> int:
        n = len(s)
        m = len(t)

        @cache
        def dfs(i, j):
            if i <0 or j < 0:
                return 0
            if s[i] == t[j]:
                return dfs(i-1,j-1) + 1
            else:
                return max(dfs(i-1, j), dfs(i, j-1))
        return dfs(n-1, m-1)
```

Input:  `abcde` and `ace`

output:

```shell
3
```

#### Complexity

- Time complexity: ( O(nm) ), where ( n ) is the length of the input string. ( m ) is the length of the target strings.
- Space complexity: ( O(m) ), where ( m ) is the length of the target string.


### 2.  DP two dim

```python
class Solution:
    def longestCommonSubsequence(self, s: str, t: str) -> int:
        n = len(s)
        m = len(t)

        f = [[0] * (m+1) for _ in range(n+1)]

        for i, x in enumerate(s):
            for j, y in enumerate(t):
                f[i+1][j+1] = f[i][j] + 1 if x == y else max(f[i][j+1], f[i+1][j]) 
        return f[n][m]
```

Input:  `abcde` and `ace`

output:

```shell
3
```
#### Complexity

- Time complexity: ( O(nm) ), where ( n ) is the length of the input string. ( m ) is the length of the target strings.
- Space complexity: ( O(m) ), where ( m ) is the length of the target string.

### 2.  DP one dim

```python
class Solution:
    def longestCommonSubsequence(self, s: str, t: str) -> int:
        n = len(s)
        m = len(t)

        f = [0] * (m+1)

        for i, x in enumerate(s):
            prev = f[0]
            for j, y in enumerate(t):
                temp = f[j+1]
                f[j+1] = prev + 1 if x == y else max(f[j+1], f[j])
                prev = temp
        
        return f[m]
```

Input:  `abcde` and `ace`

output:

```shell
3
```

#### Complexity

- Time complexity: ( O(nm) ), where ( n ) is the length of the input string. ( m ) is the length of the target strings.
- Space complexity: ( O(m) ), where ( m ) is the length of the target string.
